---
layout: default
title: AP Questions with soln
nav_order: 9
description: ""
has_children: true
parent: Index MSET
grand_parent: Home
tags: [MathJax, Mathematic]
mathjax: true
---
# ðŸ“˜ Arithmetic Progression â€“ JEE Mains Practice Questions with Solutions

---

## ðŸ§® Question Set (Medium to Hard)

---

### **Q1.**
If the sum of the first $n$ terms of an arithmetic progression is $S_n = 3n^2 + 5n$, then the $k^{\text{th}}$ term ($a_k$) is:

A) $6k + 2$  
B) $6k + 5$  
C) $6k - 1$  
D) $3k + 5$

**Solution:**  
$a_k = S_k - S_{k-1} = (3k^2 + 5k) - [3(k-1)^2 + 5(k-1)] = 6k + 2.$  
âœ… **Answer:** $a_k = 6k + 2$

---

### **Q2.**
In an A.P., the sum of the first 20 terms is zero and the first term is 10. The common difference $d$ is:

A) $-1$  
B) $-\dfrac{19}{2}$  
C) $-1.05$  
D) $-\dfrac{20}{19}$

**Solution:**  
$S_n = \dfrac{n}{2}[2a + (n-1)d]$  
$\Rightarrow 0 = 10[20 + 19d] \Rightarrow d = -\dfrac{20}{19}.$  
âœ… **Answer:** $d = -\dfrac{20}{19}$

---

### **Q3.**
The 5th term of an A.P. is 10 and the 15th term is 50. The sum of its first 20 terms is:

A) 400  
B) 600  
C) 800  
D) 900

**Solution:**  
$a + 4d = 10,\ a + 14d = 50 \Rightarrow 10d = 40 \Rightarrow d = 4.$  
Then $a = 10 - 16 = -6.$  
$S_{20} = \dfrac{20}{2}[2a + 19d] = 10(-12 + 76) = 640.$  
âœ… **Answer:** $S_{20} = 640$ *(None of the options match exactly.)*

---

### **Q4.**
If $\dfrac{S_n}{S_m} = \dfrac{n^2}{m^2}$ for an A.P., then find $\dfrac{a_n}{a_m}$.

A) $\dfrac{n}{m}$  
B) $\dfrac{n^2}{m^2}$  
C) $\dfrac{2n-1}{2m-1}$  
D) $\dfrac{2n+1}{2m+1}$

**Solution:**  
$S_n = \dfrac{n}{2}[2a + (n-1)d].$  
For $\dfrac{S_n}{S_m} = \dfrac{n^2}{m^2}$ to hold, the linear term must vanish: $2a - d = 0 \Rightarrow d = 2a.$  
Then $a_n = a + (n-1)d = (2n - 1)a.$  
Hence $\dfrac{a_n}{a_m} = \dfrac{2n - 1}{2m - 1}.$  
âœ… **Answer:** $\dfrac{2n - 1}{2m - 1}$

---

### **Q5.**
If $a, b, c, d$ are in A.P., then evaluate $(b^2 - ac) + (c^2 - bd)$.

A) 0  
B) $ad - bc$  
C) $(b-c)^2$  
D) $2d^2$

**Solution:**  
Let $b = a + d,\ c = a + 2d,\ d = a + 3d.$  
Then $b^2 - ac = d^2,$ and $c^2 - bd = d^2.$  
Sum $= 2d^2.$  
âœ… **Answer:** $2d^2$

---

### **Q6.**
The arithmetic mean of the squares of the first $n$ natural numbers equals the square of their arithmetic mean if and only if $n =$

A) 1  
B) 2  
C) 3  
D) None

**Solution:**  
$\dfrac{1^2 + 2^2 + \dots + n^2}{n} = \left(\dfrac{n+1}{2}\right)^2$  
$\Rightarrow \dfrac{(n+1)(2n+1)}{6} = \dfrac{(n+1)^2}{4}$  
$\Rightarrow 4(2n + 1) = 6(n + 1) \Rightarrow n = 1.$  
âœ… **Answer:** $n = 1$

---

### **Q7.**
The sum of three numbers in A.P. is 15, and their product is 80. The numbers are:

A) 2, 5, 8  
B) 3, 5, 7  
C) 4, 5, 6  
D) None of these

**Solution:**  
Let numbers = $(a - d),\ a,\ (a + d).$  
$3a = 15 \Rightarrow a = 5.$  
$a(a^2 - d^2) = 80 \Rightarrow 5(25 - d^2) = 80 \Rightarrow d^2 = 9 \Rightarrow d = 3.$  
Numbers: $2, 5, 8.$  
âœ… **Answer:** $2, 5, 8$

---

### **Q8.**
If $S_n = n(7n + 1)$, find the 20th term.

A) 279  
B) 281  
C) 283  
D) 285

**Solution:**  
$a_n = S_n - S_{n-1} = [7n^2 + n] - [7(n-1)^2 + (n-1)]$  
$= 7n^2 + n - (7n^2 - 14n + 6 + n - 1) = 14n - 6.$  
$a_{20} = 14(20) - 6 = 274.$  
âœ… **Answer:** $a_{20} = 274$

---

### **Q9.**
The A.P. has its first term $a = 5$ and the 5th term equals one-fourth of the 20th term. Find the 15th term.

A) 45  
B) 60  
C) 65  
D) 75

**Solution:**  
$a_5 = a + 4d = \dfrac{1}{4}(a + 19d).$  
$5 + 4d = \dfrac{1}{4}(5 + 19d)$  
$\Rightarrow 20 + 16d = 5 + 19d \Rightarrow d = 5.$  
$a_{15} = a + 14d = 5 + 70 = 75.$  
âœ… **Answer:** $75$

---

### **Q10.**
Let $a_1, a_2, a_3, \dots$ be an A.P. If $a_p = q$ and $a_q = p$, then the sum of the first $(p + q)$ terms is:

A) $(p + q)a_1$  
B) $\dfrac{(p + q)}{2}(p + q)$  
C) $(p + q)$  
D) $\dfrac{(p + q)}{2}[2a_1 + (p + q - 1)d]$

**Solution:**  
$a_p = a_1 + (p - 1)d = q,$  
$a_q = a_1 + (q - 1)d = p.$  
Subtracting: $(p - q)d = q - p \Rightarrow d = -1.$  
Then $a_1 = q + p - 1.$  
Sum of $(p + q)$ terms:  
$$
S_{p+q} = \frac{p + q}{2}[2a_1 + (p + q - 1)d]
= \frac{p + q}{2}[2(p + q - 1) - (p + q - 1)]
= \frac{(p + q)(p + q - 1)}{2}.
$$  
âœ… **Answer:** $\dfrac{(p + q)(p + q - 1)}{2}$

---

**End of Solutions**
