1
Sequence and
Series

ARITHMATIC PROGRESSION (A.P.)
KEY FACTS
1. A sequence is a set of numbers specified in a definite order by some assigned rule or law.

Ex. 2, 7, 12, 17.... (Each succeeding term is obtained by adding 5 to the preceding term)
$1,2,4,8,16 \ldots$.
(Each succeeding term is obtained by multiplying the preceding term by 2 )
A finite sequence is that which ends or has a last term.
Ex. 5, 9, 13, 17, 21.
An infinite sequence is one which has no last term.
Ex. 3, 6, 12, 24, 48....
In general, $\boldsymbol{a}_{\boldsymbol{n}}$ or $\boldsymbol{T}_{\boldsymbol{n}}$ denotes the $\boldsymbol{n}$ th term of a sequence.
2. An expression consisting of the term of a sequence, alternating with the symbol ' + ' is called a series.

Ex. The sequence $\frac{2}{3}, \frac{4}{5}, \frac{6}{7}, \ldots$ expressed as a series is $\frac{2}{3}+\frac{4}{5}+\frac{6}{7}+\ldots$.
3. Arithmetic Progression (A.P.): A sequence is called an arithmetic progression if its terms continually increase or decrease by the same number. The fixed number by which they increase or decrease is called the common difference. Three quantities $a, b, c$ will be in A.P. if $b-a=c-b$, i.e., $\mathbf{2} \boldsymbol{b}=\boldsymbol{a}+\boldsymbol{c}$.
(a) $n$th term of an A.P.: The $n$th term of an A.P. $a, a+d, a+2 d, a+3 d, \ldots$ is

$$
T_n=a+(n-1) d
$$

where $\boldsymbol{T}_{\boldsymbol{n}}$ denotes $n$th term, $\boldsymbol{a}$ the first term, $\boldsymbol{n}$ the number of terms and $\boldsymbol{d}$ the common difference.
Also, common difference $\boldsymbol{d}=\boldsymbol{T}_n-\boldsymbol{T}_{n-1}$.
Ex. The 9th term of the A.P.: 2, $5,8 \ldots$. is

$$
T_9=2+(9-1) \times 3=2+24=\mathbf{2 6} .
$$


Note: Here $a=2, d=3$.
(b) Sum of $\boldsymbol{n}$ terms of an A.P.

Let the A.P. be $a, a+d, a+2 d, \ldots$ Let $l$ be the last term and $S$ the required sum. Then,

$$
\begin{aligned}
\boldsymbol{S} & =\frac{\boldsymbol{n}}{\mathbf{2}}(\boldsymbol{a}+\boldsymbol{l})=\frac{\text { Number of terms }}{2}(\text { First term }+ \text { Last term }) \\
& =\frac{n}{2}(a+a+(n-1) d)=\frac{n}{2}(2 a+(n-1) d)
\end{aligned}
$$

where $n$ is the number of terms, $a$ is first term and $d$ is common difference.
Also, $\quad n$th term $=$ Sum of $n$ terms - Sum of $(n-1)$ terms
i.e.,

$$
T_n=S_n-S_{n-1} .
$$

Ex. The sum of 20 terms of the the A.P. $1,3,5,7,9 \ldots$ is

$$
\begin{aligned}
S_{20} & =\frac{20}{2}(2 \times 1+(20-1) \times 2) \quad(\because a=1, d=2, n=20) \\
& =10 \times 40=400 .
\end{aligned}
$$

(c) Arithmetic Mean: The Arithmetic Mean between two numbers is the number which when placed between them forms an arithmetic progression with them. Thus if $\boldsymbol{x}$ is the arithmetic mean of two given numbers $\boldsymbol{a}$ and $\boldsymbol{b}$, then $a, x, b$ form an A.P.

$$
\therefore \quad x-a=b-x \quad \Rightarrow \boldsymbol{x}=\frac{\boldsymbol{a}+\boldsymbol{b}}{\mathbf{2}}
$$


Ex. (a) The arithmetic mean between -4 and 6 is $\frac{6+(-4)}{2}=\mathbf{1}$.
(b) Find 4 arithmetic means between 3 and 23.

Let $A_1, A_2, A_3, A_4$, be the four arithmetic means between 3 and 23 .
Then, $3, A_1, A_2, A_3, A_4, 23$ form an A.P.
Here, First term $=a=3$
Sixth term $=T_6=23$
Number of terms $=n=6$
Common difference $=d=$ ?

$$
\begin{aligned}
T_6 & =a+(n-1) \times d \\
\Rightarrow 23 & =3+(6-1) \times d \\
\Rightarrow 23 & =3+5 d \Rightarrow 5 d=20 \Rightarrow d=\mathbf{4} \\
\therefore \quad A_1 & =3+4=7, A_2=7+4=11, A_3=11+4=15, A_4=15+4=19
\end{aligned}
$$

(d) Some useful facts about an A.P.
I. If each term of a given A.P. is increased or decreased or multiplied or divided by the same number, the resulting progression is also an A.P.
II. If $a, b, c$ are in A.P., then $\frac{a-b}{b-c}=1$, i.e., $\frac{\text { First term }- \text { Second term }}{\text { Second term }- \text { Third term }}=1$.
(e) If we have to find an odd number of terms in A.P. whose sum is given, it is convenient to take $a$ as the middle term and $d$ as the common difference. Thus, three terms may by taken as $\boldsymbol{a}-\boldsymbol{d}, \boldsymbol{a}, \boldsymbol{a}+\boldsymbol{d}$ and five terms as $\boldsymbol{a}-\mathbf{2} \boldsymbol{d}, \boldsymbol{a}-\boldsymbol{d}, \boldsymbol{a}, \boldsymbol{a}+\boldsymbol{d}, \boldsymbol{a}+\mathbf{2} \boldsymbol{d}$. [Solved Ex. 13, 14]. If we have to find even number of terms, we take $a-d, a+d$ as the middle terms and $2 d$ as the common difference. Then, four terms are taken as $\boldsymbol{a}-\mathbf{3} \boldsymbol{d}, \boldsymbol{a}-\boldsymbol{d}, \boldsymbol{a}+\boldsymbol{d}, \boldsymbol{a}+\mathbf{3} \boldsymbol{d}$.

SOLVED EXAMPLES

Ex. 1. The 8th term of a series in A.P. is 23 and the 102 th term is 305 . Find the series.
Sol. Let $a$ be the first term and $d$ be the common difference.

$$
\begin{aligned}
& \text { Then, } \quad T_8=a+(8-1) d \quad \Rightarrow \quad 23=a+7 d \\
& T_{102}=a+(102-1) d \quad \Rightarrow \quad 305=a+101 d \\
& \therefore \text { Eqn (ii) }- \text { Eqn (i) } \\
& \Rightarrow \quad 94 d=282 \quad \Rightarrow \quad d=3
\end{aligned}
$$


Now substituting $d=3$ in (i), we get $23=a+21 \Rightarrow a=2$.

$$
\therefore \quad a=2, d=3 \Rightarrow \text { Series is } 2+5+8+11+\ldots . .
$$


Ex. 2. If $\boldsymbol{a}, \boldsymbol{b}$ and $\boldsymbol{c}$ be respectively the $\boldsymbol{p}$ th, $\boldsymbol{q}$ th and $\boldsymbol{r}$ th terms of an A.P., prove that $\boldsymbol{a}(\boldsymbol{q}-\boldsymbol{r})+\boldsymbol{b}(\boldsymbol{r}-\boldsymbol{p})+\boldsymbol{c}(\boldsymbol{p}-\boldsymbol{q})=\mathbf{0}$.
Sol. Let $A$ be the first term and $D$ the common difference of the given A.P.
Then,

$$
\begin{aligned}
& T_p=A+(p-1) \mathrm{D}=a \\
& T_q=A+(q-1) D=b \\
& T_r=A+(r-1) D=c
\end{aligned}
$$


$$
\begin{aligned}
& \therefore(i) \times(q-r)+(i i) \times(r-p)+(i i i) \times(p-q) \\
& \Rightarrow A[(q-r)+(r-p)+(p-q)]+D[(p-1)(q-r)+(q-1)(r-p)+(r-1)(p-q)] \\
& \quad=a(q-r)+b(r-p)+c(p-q) \\
& \Rightarrow A[0]+D[p q-q-p r+r+q r-r-p q+p+p r-p-q r+q]=a(q-r)+b(r-p)+c(p-q)
\end{aligned}
$$

Ex. 3. Which term of the progression $19,18 \frac{1}{5}, 17 \frac{2}{5}, \ldots .$. is the first negative term?
Sol. Here $a=19, d=18 \frac{1}{5}-19=-\frac{4}{5}$
Let the $n$th term be the first negative term. Then,

$$
\begin{aligned}
T_n<0 & \Rightarrow a+(n-1) d<0 \\
& \Rightarrow 19+(n-1)(-4 / 5)<0 \\
& \Rightarrow 19-\frac{4}{5} n+\frac{4}{5}<0 \\
& \Rightarrow \frac{99}{5}-\frac{4}{5} n<0 \Rightarrow n>\frac{99}{5} \times \frac{5}{4} \Rightarrow n>\frac{99}{4}=24 \frac{3}{4} \\
& \Rightarrow n=\mathbf{2 5}
\end{aligned}
$$


Ex. 4. Find the sum of the series $\mathbf{1 0 1}+\mathbf{9 9}+\mathbf{9 7}+\ldots .+\mathbf{4 7}$.
Sol. In this case, we have to first find the number of terms.
Here $a=101, l=T_n=47, d=99-101=-2$
$\therefore \quad 47=101+(n-1) \times(-2)$, where $n=$ number of terms

$$
\begin{aligned}
& \Rightarrow 47=101-2 n+2 \\
& \Rightarrow 2 n=103-47=56 \Rightarrow n=28 \\
& \therefore S_n=\frac{n}{2}(a+l) \\
& \Rightarrow S_{28}=\frac{28}{2}(101+47)=14 \times 148=\mathbf{2 0 7 2}
\end{aligned}
$$


Ex. 5. The sums of $n$ terms of two arithmetic series are in the ratio $2 n+1: 2 n-1$. Find the ratio of their 10 th terms.

Sol. Let the two arithmetic series be $a, a+d, a+2 d \ldots$. and $A, A+D, A+2 D, \ldots$.
Given that, $\frac{n / 2[2 a+(n-1) d]}{n / 2[2 A+(n-1) D]}=\frac{2 n+1}{2 n-1}$

$$
\Rightarrow \frac{2 a+(n-1) d}{2 A+(n-1) D}=\frac{2 n+1}{2 n-1}
$$


Ratio of the 10 th terms of these series $=\frac{t_{10}}{T_{10}}=\frac{a+9 d}{A+9 D}=\frac{2 a+18 d}{2 A+18 D}$
$\therefore \quad$ Putting $n=19$ in (i), we have $\frac{t_{10}}{T_{10}}=\frac{2 a+18 d}{2 A+18 D}=\frac{2 \times 19+1}{2 \times 19-1}=\frac{\mathbf{3 9}}{\mathbf{3 7}}$.

Ex. 6. The sum of the first $n$ terms of the arithmetical progression $3,5 \frac{1}{2}, 8, \ldots$ is equal to the $2 n$th term of the A.P. $16 \frac{1}{2}, 28 \frac{1}{2}, 40 \frac{1}{2}, \ldots$. Calculate the value of $n$.

Ch 1-4
IIT FOUNDATION MATHEMATICS CLASS - X

Sol. For the A.P. : $3,5 \frac{1}{2}, 8, \ldots . \quad a=3, d=2 \frac{1}{2}$, number of terms $=n$

$$
\Rightarrow \quad S_n=\frac{n}{2}[2 a+(n-1) d]=\frac{n}{2}\left(6+(n-1) \times \frac{5}{2}\right)
$$


For the A.P.: $16 \frac{1}{2}, 28 \frac{1}{2}, 40 \frac{1}{2} \ldots \quad a=16 \frac{1}{2}, d=12$.

$$
\therefore \quad T_{2 n}=a+(2 n-1) d=16 \frac{1}{2}+(2 n-1) \times 12
$$


Given, $S_n=T_{2 n} \Rightarrow \frac{n}{2}\left(6+(n-1) \frac{5}{2}\right)=\frac{33}{2}+(2 n-1) \times 12$
(From (i) and (ii))

$$
\begin{array}{ll}
\Rightarrow \frac{6 n}{2}+\frac{5 n^2}{4}-\frac{5 n}{4}=\frac{33}{2}+24 n-12 & \Rightarrow \frac{7 n}{4}+\frac{5 n^2}{4}=\frac{9}{2}+24 n \\
\Rightarrow \frac{5 n^2}{4}-\frac{89 n}{4}-\frac{9}{2}=0 & \Rightarrow 5 n^2-89 n-18=0 \\
\Rightarrow 5 n^2-90 n+n-18=0 & \Rightarrow 5 n(n-18)+1(n-18)=0 \\
\Rightarrow(n-18)(5 n+1)=0 & \Rightarrow n=18 \text { or }-\frac{1}{5}
\end{array}
$$

$\Rightarrow$ Neglecting $-v e$ value, we have $n=\mathbf{1 8}$.

Ex. 7. Let $a_1, a_2, a_3$, be the terms of an A.P. If $\frac{a_1+a_2+a_3+\ldots .+a_p}{a_1+a_2+a_3+\ldots .+a_q}=\frac{p^2}{q^2}(p \neq q)$, then find $\frac{a_6}{a_{21}}$.
(AIEEE 2006)

Sol. Let $d$ be the common difference for the A.P.; $a_1, a_2, a_3, \ldots$.
Then, $\frac{S_p}{S_q}=\frac{p / 2\left[2 a_1+(p-1) d\right]}{q / 2\left[2 a_1+(q-1) d\right]}=\frac{p^2}{q^2}$
$\Rightarrow \frac{2 a_1+(p-1) d}{2 a_1+(q-1) d}=\frac{p}{q}$

$$
\Rightarrow \quad q\left[2 a_1+(p-1) d\right]=p\left[2 a_1+(q-1) d\right]
$$

$\Rightarrow 2 a_1 q+p q d-q d=2 a_1 p+p q d-p d$
$\Rightarrow p d-q d=2 a_1 p-2 a_1 q$
$\Rightarrow d(p-q)=2 a_1(p-q)$
$\Rightarrow d=2 a_1$
Now $\frac{\text { Term } 6}{\text { Term } 21}=\frac{a_6}{a_{21}}=\frac{a_1+(6-1) d}{a_1+(21-1) d}=\frac{a_1+5 \times 2 a_1}{a_1+20 \times 2 a_1}=\frac{11 a_1}{41 a_1}=\frac{\mathbf{1 1}}{\mathbf{4 1}}$.
Ex. 8. If the number of terms of an A.P. is $(2 n+1)$, then what is the ratio of the sum of the odd terms to the sum of even terms?
(NDA/NA 2008)
Sol. Let the A.P. be $a, a+d, a+2 d, \ldots, a+(2 n-1) d, a+2 n d$
Then, the progression of odd terms is $a, a+2 d, a+4 d, \ldots, a+2 n d$.
This progression has ( $n+1$ ) terms.

$$
\text { Its sum }=\frac{n+1}{2}[a+a+2 n d]=\frac{n+1}{2}[2 a+2 n d]=(n+1)(a+n d)
$$


The progression of even terms is $a+d, a+3 d, \ldots \ldots a+(2 n-1) d$.
This progression has $n$ terms.

$$
\text { Its sum }=\frac{n}{2}\left[(a+d)+(a+(2 n-1) d]=\frac{n}{2}[2 a+2 n d]=n(a+n d)\right.
$$


$$
\therefore \quad \frac{\text { Sum of odd terms }}{\text { Sum of even terms }}=\frac{(n+1)(a+n d)}{n(a+n d)}=\frac{\boldsymbol{n}+\mathbf{1}}{\boldsymbol{n}} .
$$

Ex. 9. If the sum of the roots of the quadratic equation $\boldsymbol{a} \boldsymbol{x}^{\mathbf{2}}+\boldsymbol{b} \boldsymbol{x}+\boldsymbol{c}=\mathbf{0}$ is equal to the sum of the squares of their reciprocals, then show that $\boldsymbol{a} \boldsymbol{b}^{\mathbf{2}}, \boldsymbol{c} \boldsymbol{a}^{\mathbf{2}}, \boldsymbol{b} \boldsymbol{c}^{\mathbf{2}}$ are in A.P.
(DCE)
Sol. Let $\alpha, \beta$ be the roots of the equation $a x^2+b x+c=0$.
Then $\alpha+\beta=-b / a, \alpha \beta=c / a$
Given, Sum of roots = Sum of squares of reciprocals of roots

$$
\begin{array}{lll}
\Rightarrow \alpha+\beta=\frac{1}{\alpha^2}+\frac{1}{\beta^2} & \Rightarrow \alpha+\beta=\frac{\alpha^2+\beta^2}{\alpha^2 \beta^2} & \Rightarrow \alpha+\beta=\frac{(\alpha+\beta)^2-2 \alpha \beta}{(\alpha \beta)^2} \\
\Rightarrow-b / a=\frac{(-b / a)^2-\frac{2 c}{a}}{(c / a)^2} & \Rightarrow-\frac{b}{a}=\frac{b^2-2 c a}{c^2} & \Rightarrow-b c^2=a b^2-2 c a^2 \\
\Rightarrow 2 c a^2=a b^2+b c^2 & \Rightarrow a b^2, c a^2, b c^2 \text { are in A.P. } & (\because a, b, c \text { in A.P. } \Rightarrow 2 b=a+c)
\end{array}
$$


Ex. 10. Find the value of $n$, if $\frac{a^{n+1}+b^{n+1}}{a^n+b^n}$ is the arithmetic mean between $a$ and $b$.
(WBJEE 2009)
Sol. The arithmetic mean between $a$ and $b$ is $\frac{a+b}{2}$.

$$
\begin{array}{ll}
\text { Given, } \frac{a+b}{2}=\frac{a^{n+1}+b^{n+1}}{a^n+b^n} & \\
\Rightarrow\left(a^n+b^n\right)(a+b)=2\left(a^{n+1}+b^{n+1}\right) & \Rightarrow a^{n+1}+a^n b+b^n a+b^{n+1}=2 a^{n+1}+2 b^{n+1} \\
\Rightarrow a^{n+1}+b^{n+1}=a^n b+b^n a & \Rightarrow\left(a^{n+1}-b a^n\right)-\left(b^n a-b^{n+1}\right)=0 \\
\Rightarrow a^n(a-b)-b^n(a-b)=0 & \Rightarrow\left(a^n-b^n\right)(a-b)=0 \\
\Rightarrow\left(a^n-b^n\right)=0 \text { or }(a-b)=0 &
\end{array}
$$


But $a \neq b \Rightarrow a-b \neq 0$

$$
\therefore a^n-b^n=0 \Rightarrow a^n=b^n \Rightarrow\left(\frac{a}{b}\right)^n=1 \Rightarrow\left(\frac{a}{b}\right)^n=\left(\frac{a}{b}\right)^0 \Rightarrow \boldsymbol{n}=\mathbf{0}
$$


Ex. 11. If $\log _{10} 2, \log _{10}\left(2^x-1\right)$ and $\log _{10}\left(2^x+3\right)$ be three consecutive terms of an A.P., then find the value of $\boldsymbol{x}$.
(AMU 2012)
Sol. Given, $\log _{10} 2, \log _{10}\left(2^x-1\right), \log _{10}\left(2^x+3\right)$ are in A.P. Then,

$$
\begin{aligned}
& \log _{10}\left(2^x-1\right)-\log _{10} 2=\log _{10}\left(2^x+3\right)-\log _{10}\left(2^x-1\right) \\
& \Rightarrow \log _{10}\left(\frac{2^x-1}{2}\right)=\log _{10}\left(\frac{2^x+3}{2^x-1}\right) \\
& \Rightarrow \frac{2^x-1}{2}=\frac{2^x+3}{2^x-1} \\
& \Rightarrow 2^{2 x}-2.2^x+1=2.2^x+6 \\
& \Rightarrow 2^{2 x}-5.2^x+2^x-5=0 \\
& \Rightarrow\left(2^x-5\right)\left(2^x+1\right)=0 \\
& \Rightarrow 2^{2 x}-4.2^x-5=0 \\
& \Rightarrow 2^x\left(2^x-5\right)+1\left(2^x-5\right)=0 \\
& \quad \Rightarrow 2^x=5 \\
& \Rightarrow x=\log _2 5
\end{aligned}
$$