---
layout: default
title: 2. Linear Equation One Variable
nav_order: 4
description: ""
has_children: false
parent:  Fiitjee Phasebook
tags: [MathJax, Mathematic]
mathjax: true
---


### LINEAR EQUATION IN ONE VARIABLE  

An equation is an equality which involves one or more unknown quantities. These quantities are known as variables.
A linear equation in one variable is that equation in which only single variable with degree one occurs. This can be written in the form $a x+b=c$, where $a, b$ and $c$ are numbers, $a \neq 0$ and $x$ is the variable.

For example, $3 x-9=4, \frac{1}{4} y+\sqrt{2}=y-1,5 x+9=0$ are linear equations in one variable.

**$\sigma$ Illustration 1:**

Which of the following equations are linear equations in one variable?
(i) $2 y-4=9+4$  
(ii) $x+\frac{1}{x}=4$  
(iii) $\frac{5}{2} x+\frac{9}{3}=2 x-5$  
(iv) $\quad(x-2)^2=x^2-4$  
(v) $(x-3)(x+2)=x+5$  

Solution:  
(i) This equation involves the variable $y$ only in the first degree. So it is a linear equation in one variable.
(ii) $x+\frac{1}{x}=4 \Rightarrow x^2+1=4 x$

This equation involves the variable $x$ in second degree. Therefore it is not a linear equation.
(iii) This equation involves variable $x$ only in the first degree and hence it is a linear equation.
(iv) We have $(x-2)^2=x^2-4 \Rightarrow x^2-4 x+4=x^2-4$

$
\Rightarrow-4 x+4=-4
$

This equation involves the variable $x$ in the first degree. So it is a linear equation in one variable.
(v)

$
\begin{aligned}
& (x-3)(x+2)=x+5 \newline
& \Rightarrow x^2-x-6=x+5
\end{aligned}
$


In this equation the variable $x$ is in second degree and hence it is not a linear equation in one variable.

*Solution of a linear equation in one variable*   
A value (real number) of the variable that satisfies the equation is called a solution or root of the equation.
For example, $x=2$ is a solution of the equation $2 x-3=x-1$, because when we put $x=2$ in the equation, we get $\operatorname{LHS}=$ RHS ( $=1$ each). Here, $x=2$ is also known as the root of the equation.

Solving of an equation  
The method of finding the roots of an equation is known as solving the equation.
Rules for solving an equation  
(i) The same quantity can be added to both sides of the equation.  
(ii) The same quantity can be subtracted from both sides of the equation.  
(iii) Both sides of the equation can be multiplied or divided by same non-zero number.  
(iv) The equation of the form $\frac{a x+b}{c x+d}=\frac{p}{q}$, where $a, b, c, d, p$ and $q$ are numbers and $c x+d \neq 0$ can be reduced to linear equation.  
$q(a x+b)=p(c x+d)$.   
This process is called cross multiplication. 

Any term of an equation may be taken to the other side with a change in its sign. This process is known as transposition. Thus $2 x+3=3 x-4 \Rightarrow 3+4=3 x-2 x$.  
*Solution by transposition*   
Step I: Transpose the term involving the variable (unknown) from RHS to the LHS and those terms which do not involve variable from LHS to RHS while transposing, the sign of the term is to be changed.  
Step II : Simplify the two sides to obtain the equation in the form of $a x=b$.  
Step III : Divide both sides of the equation by the coefficient of $x$.  

**$\sigma$ Illustration 2:**

Solve the following equations and check your answer:  
(i) $\frac{3}{4} x+\frac{5}{2} x=\frac{6}{5} x-7$  
(ii) $\frac{x}{2 x-4}=\frac{x-4}{2 x}, x \in Q, x \neq 0, x \neq 2$  
(iii) $(6 x-5)(2 x+4)-3(2 x-3)^2=53$  
(iv) $\frac{3}{x-1}+\frac{4}{x-2}=\frac{7}{x-3}, x \in R, x \neq 1, x \neq 2, x \neq 3$  
(v) $\frac{y^2+3}{y^2-5}=\frac{7}{5}, y \in R, y \neq \pm \sqrt{5}$  

Solution:  
(i) The given equation is $\frac{3}{4} x+\frac{5}{2} x=\frac{6}{5} x-7$  
$\Rightarrow \frac{3}{4} x+\frac{5}{2} x-\frac{6}{5} x=-7$  
(By transposition)  
$\Rightarrow 15 x+50 x-24 x=-140$  
$\Rightarrow 41 x=-140$   
(Multiplying both sides by 20, the LCM of $4,2,5$ )  
$\Rightarrow x=-\frac{140}{41}$  
(Dividing both sides by 41)  

Check:
When we put $x=-\frac{140}{41}$, we get  
LHS $=\frac{3}{4}\left(-\frac{140}{41}\right)+\frac{5}{2}\left(-\frac{140}{41}\right)=-\frac{455}{41}$  
and RHS $=\frac{6}{5}\left(-\frac{140}{41}\right)-7=-\frac{455}{41}$.  
$\therefore$ LHS $=$ RHS  
Hence $x=-\frac{140}{41}$ is a solution of the given equation.    

(ii) The equation is $\frac{x}{2 x-4}=\frac{x-4}{2 x}$  
$\Rightarrow x(2 x)=(2 x-4)(x-4)$  
(By cross multiplication)  
$\Rightarrow 2 x^2=2 x^2-12 x+16$  
$\Rightarrow 2 x^2-2 x^2+12 x=16$   
(By transposition)  
$\Rightarrow 12 x=16 \Rightarrow x=\frac{16}{12}=\frac{4}{3}$
(dividing both sides by 12)  
Check:  
When we put $x=\frac{4}{3}$ in the equation, we get  
LHS $=\frac{\frac{4}{3}}{2 \times \frac{4}{3}-4}=-1$ and $R H S=\frac{\frac{4}{3}-4}{2 \times \frac{4}{3}}=-1$.  
$\therefore$ LHS $=$ RHS  
Hence $x=\frac{4}{3}$ is the solution.  

(iii) The equation is $(6 x-5)(2 x+4)-3(2 x-3)^2=53$  
$\Rightarrow 12 x^2-10 x+24 x-20-3\left(4 x^2-12 x+9\right)=53$  
$\Rightarrow 12 x^2+14 x-20-12 x^2+36 x-27=53$  
$\Rightarrow 50 x=53+20+27=100$  
(By transposition)  
$\therefore \mathrm{x}=\frac{100}{50}$
(Dividing both sides by 50 )
$=2$
Check:
Putting $x=2$ in the equation, we get

$
\text { LHS }=7 \times 8-3=53=\text { RHS }
$

$\therefore x=2$ is the solution of given equation.  

(iv) The given equation is $\frac{3}{x-1}+\frac{4}{x-2}=\frac{7}{x-3}$
$
\begin{aligned}
& \Rightarrow \frac{3(x-2)+4(x-1)}{(x-1)(x-2)}=\frac{7}{x-3} \newline
& \Rightarrow \frac{3 x-6+4 x-4}{x^2-3 x+2}=\frac{7}{x-3}
\end{aligned}
$


$
\begin{aligned}
& \Rightarrow \frac{7 x-10}{x^2-3 x+2}=\frac{7}{x-3} \\
& \Rightarrow(x-3)(7 x-10)=7\left(x^2-3 x+2\right) \\
& \Rightarrow 7 x^2-31 x+30=7 x^2-21 x+14 \\
& \Rightarrow 7 x^2-7 x^2-31 x+21 x=14-30 \\
& \Rightarrow-10 x=-16 \\
& \Rightarrow x=\frac{-16}{-10}=\frac{8}{5}
\end{aligned}
$

(By cross multiplication)
(By transposition)

Check:
When we put $x=\frac{8}{5}$ in the equation, we get

$$
\text { LHS }=\frac{3}{\frac{8}{5}-1}+\frac{4}{\frac{8}{5}-2}=-5
$$

and RHS $=\frac{7}{\frac{8}{5}-3}=-5$.
$\therefore x=\frac{8}{5}$ is the solution.

$
\begin{aligned}
& \text { (v) We have } \frac{y^2+3}{y^2-5}=\frac{7}{5} \\
& \Rightarrow 5\left(y^2+3\right)=7\left(y^2-5\right) \\
& \Rightarrow 5 y^2+15=7 y^2-35 \\
& \Rightarrow 5 y^2-7 y^2=-35-15 \\
& \Rightarrow-2 y^2=-50 \\
& \Rightarrow y^2=\frac{-50}{-2}=25 \Rightarrow y= \pm 5
\end{aligned}
$

(By cross multiplication)
(By transposition)

Check:
When we put $y=5$ or -5 , we get LHS $=\frac{28}{20}=\frac{7}{5}=$ RHS .
$\therefore$ There are two solutions of the given equation viz $y=5$ or -5 .

Exercise 1:  
(i) Which of the following equations are linear equations?  
  (a) $\frac{3}{2} x+\frac{7}{5} x-\frac{5}{9}=\frac{5 x-3}{6}$  
  (b) $x+4=x^2-7 x+3$  
  (c) $(x-3)(x+5)=(4-x)(7-x)$  
  (d) $x+4=2 \sqrt{3}-5$  

(ii) Solve the following equations and verify their solutions:  
  (a) $0.5 x-7=0.25 x-\frac{x}{3}$  
  (b) $\frac{x}{7}-\frac{x}{14}=\frac{x}{28}+\frac{1}{4} \sqrt{3}$  
  (c) $(2 x+3)^2=(x+1)(4 x-3)-21$  
  (d) $\frac{4}{x-2}+\frac{3}{x-1}=\frac{7}{x-3}, x \neq 1,2,3$  


### Applications of linear equations
Here, we shall solve some simple word problems of daily life.
Method
Step I: Read the problem carefully.  
Step II: Denote the required quantity by $x$ (say).  
Step III: From the conditions given in the question, construct a linear equation in $x$.  
Step IV: Solve this linear equation to get the value of $x$.  

Note: If there are more than one unknown quantities, write one as $x$ and other in terms of $x$.  

**$\sigma$ Illustration 3**:
Find the three consecutive numbers such that twice the first, 3 times the second and 4 times the third together make 191.

Solution: Let the three consecutive numbers be $\mathrm{x}, \mathrm{x}+1, \mathrm{x}+2$.
Twice the number $=2 x$
3 times the second number $=3(x+1)$
4 times the third number $=4(x+2)$
$\therefore$ according to question,

$
\begin{aligned}
& 2 x+3(x+1)+4(x+2)=191 \\
& 2 x+3 x+3+4 x+8=191 \\
& 9 x=191-11=180 \\
& x=20
\end{aligned}
$

$\therefore$ the three consecutive numbers are 20, 21 and 22 .

**$\sigma$ Illustration 4**:
The sum of ages of father and son is 48 years. The quotient obtained by dividing the age of the son by the age of the father is $\frac{1}{5}$. Find their ages and verify the answer.

Solution: $\quad$ Suppose age of father $=x$ years
Age of son $=(48-x)$ years
According to question,

$
\begin{array}{ll} 
& \frac{48-x}{x}=\frac{1}{5} \\
\Rightarrow & 5(48-x)=x \\
\Rightarrow & 240-5 x=x \\
\Rightarrow & -5 x-x=-240 \\
\Rightarrow & -6 x=-240 \\
& x=\frac{240}{6} \\
& x=40
\end{array}
$

$\therefore \quad$ father's age $=40$ years

and son's age $=(48-40)=8$ years
Verification: $\frac{\text { age of son }}{\text { age of father }}=\frac{8}{40}=\frac{1}{5}$, which satisfies the condition given in question

### Exercise 2:16  
(i) A number consists of two digits. The digit in ten's place exceeds the digit in unit's place by 2 . The difference of the digits is $\frac{1}{32}$ of the number. Find the number.  
(ii) The denominator of a fraction is 1 more than its numerator. If 15 is subtracted from both the numerator and denominator, the fraction becomes $\frac{9}{10}$. Find the fraction.   
(iii) A steamer going down stream in a river, covers the distance between two towns in 20 hours. Coming back upstream, it covers this distance in 25 hours. The speed of water is 4 kmh . Find the distance between two towns.  
(iv) The perimeter of a rectangle is 240 cm . If its length is decreased by $10 \%$ and breadth is increased by $20 \%$, we get the same perimeter. Find the length and breadth of the rectangle.  
(v) The angle $A$ of a triangle $A B C$ is equal to the sum of the other two angles. Also, the ratio of the angle $B$ to the angle $C$ is $2: 3$. Determine the three angles.  

